IMP-/IMP_To_IMP-/Binary_Operations.thy
@@ -43,6 +43,15 @@ next
   thus ?case using ta_def Cons seq_terminates_iff by fastforce
 qed
 
+thm_oracles t_small_step_fun_com_list_to_seq_terminates
+
+declare seq_terminates_when'[intro]
+lemma tsmall_seq [intro]: "
+  t_small_step_fun t1 (c1, s1) = (SKIP, s2) \<Longrightarrow>
+  t_small_step_fun t2 (c2, s2) = (SKIP, s3) \<Longrightarrow> 
+t_small_step_fun (t1+t2+1) (c1;;c2, s1) = (SKIP, s3)"
+  by (meson less_add_one seq_terminates_when')
+
 lemma com_list_to_seq_of_length_one_terminates_iff:
   "t_small_step_fun t (com_list_to_seq [c], s1) = (SKIP, s2) \<longleftrightarrow>
   (t > 0 \<and> t_small_step_fun (t - 1) (c, s1) = (SKIP, s2))"
@@ -55,13 +64,28 @@ lemma com_list_to_seq_variables: "set (enumerate_variables (com_list_to_seq cs))
   apply(induction cs)
   by(auto simp: set_enumerate_variables_seq)
 
-fun binary_assign_constant:: "nat \<Rightarrow> vname \<Rightarrow> nat \<Rightarrow> IMP_Minus_com" where
-"binary_assign_constant 0 v x = SKIP" |
-"binary_assign_constant (Suc n) v x = (var_bit_to_var (v, n)) ::= nth_bit x n ;;
-  binary_assign_constant n v x"
+text \<open>Computing enumerate_variables is too slow for the _anything_, this does it quickly:\<close>
+fun lvarS :: "com \<Rightarrow> vname set" where
+  "lvarS (Assign v _) = {v}" |
+  "lvarS (c1;;c2) = lvarS c1 \<union> lvarS c2" |
+  "lvarS (If v c1 c2) = {v} \<union> lvarS c1 \<union>lvarS c2" |
+  "lvarS (While v c) = {v} \<union> lvarS c" |
+  "lvarS _ = {}"
 
-lemma result_of_binary_assign_constant: "t_small_step_fun (3 * n)
-  (binary_assign_constant n v x, s)
+lemma larvs_set_enum: "lvarS c = set (enumerate_variables c)"
+  apply (induction c) 
+  apply simp_all
+  using set_enumerate_variables_seq apply presburger
+  using set_enumerate_variables_if apply auto[1]
+  using set_enumerate_variables_while by auto
+
+fun binary_assign_constant_bits:: "nat \<Rightarrow> vname \<Rightarrow> nat \<Rightarrow> IMP_Minus_com" where
+"binary_assign_constant_bits 0 v x = SKIP" |
+"binary_assign_constant_bits (Suc n) v x = (var_bit_to_var (v, n)) ::= nth_bit x n ;;
+  binary_assign_constant_bits n v x"
+
+lemma result_of_binary_assign_constant_bits: "t_small_step_fun (3 * n)
+  (binary_assign_constant_bits n v x, s)
   = (SKIP, \<lambda>w. (case var_to_var_bit w of
       Some (w', m) \<Rightarrow> (if w' = v \<and> m < n then Some (nth_bit x m) else s w) |
       _ \<Rightarrow> s w))"
@@ -74,27 +98,71 @@ proof(induction n arbitrary: s)
     by(auto simp: fun_eq_iff var_to_var_bit_eq_Some_iff  split: option.splits)
 qed (auto simp: fun_eq_iff split: option.splits)
 
-lemma binary_assign_constant_variables: "set (enumerate_variables (binary_assign_constant n v x))
-  = { var_bit_to_var (v, i) | i. i < n }"
+lemma binary_assign_constant_bits_variables[simp]: 
+  "set (enumerate_variables (binary_assign_constant_bits n v x)) = { var_bit_to_var (v, i) | i. i < n }"
   apply(induction n)
   by(auto simp: set_enumerate_variables_seq)
 
+definition binary_assign_zero :: "nat \<Rightarrow> vname \<Rightarrow> nat \<Rightarrow> IMP_Minus_com" where
+"binary_assign_zero n v x = (var_bit_to_var (v, n)) ::= zero_bit x n"
+
+lemma result_of_binary_assign_zero: "t_small_step_fun 1
+  (binary_assign_zero n v x, s) 
+  = (SKIP, \<lambda>w. (case var_to_var_bit w of
+      Some (w',m) \<Rightarrow> (if w' = v \<and> m = n then Some (zero_bit x m) else s w ) | _ \<Rightarrow> s w))"
+  unfolding binary_assign_zero_def
+  by (auto simp: numeral_eq_Suc var_to_var_bit_eq_Some_iff fun_eq_iff split: option.splits)
+
+lemma binary_assign_zero_vars: "enumerate_variables (binary_assign_zero n v x) = [var_bit_to_var (v,n)]"
+  unfolding binary_assign_zero_def by simp
+
+definition "binary_assign_constant n v x = binary_assign_zero n v x;; binary_assign_constant_bits n v x"
+declare [[names_short]]
+
+lemma binary_assign_constant_ne_Skip[simp]: "binary_assign_constant n v x \<noteq> SKIP"
+  unfolding binary_assign_constant_def by auto
+
+lemma result_of_binary_assign_constant:
+  "t_small_step_fun (3 * n + 2)
+  (binary_assign_constant n v x, s)
+  = (SKIP, \<lambda>w. (case var_to_var_bit w of
+      Some (w', m) \<Rightarrow> (if w' = v \<and> m < n then Some (nth_bit x m) else if w' = v \<and> m = n then Some (zero_bit x m) else s w) |
+      _ \<Rightarrow> s w))"
+  unfolding binary_assign_constant_def
+  apply (rule seq_terminates_when[of 1 "3*n"])
+  apply simp
+   apply (rule result_of_binary_assign_zero)
+  apply (subst result_of_binary_assign_constant_bits[of n v x])
+  by (auto simp add: fun_eq_iff split: option.splits if_splits)
+
+lemma binary_assign_constant_variables[simp]: "set (enumerate_variables (binary_assign_constant n v x))
+  = {var_bit_to_var (v, i) | i. i < n} \<union> { var_bit_to_var (v, n)}"
+  apply (subst larvs_set_enum[symmetric]) 
+  unfolding binary_assign_constant_def binary_assign_zero_def
+  apply auto
+   apply (auto simp add: larvs_set_enum)
+  done
+
 lemma result_of_binary_assign_constant_on_translated_state_aux:
   assumes "n > 0"
-  shows "t_small_step_fun (3 * n) (binary_assign_constant n v x,
+  shows "t_small_step_fun (3 * n+2) (binary_assign_constant n v x,
     IMP_State_To_IMP_Minus s n)
     = (SKIP, IMP_State_To_IMP_Minus (s(v := x)) n)"
-  apply(subst result_of_binary_assign_constant)
-  using assms
-  by (auto simp: fun_eq_iff IMP_State_To_IMP_Minus_def
-      IMP_State_To_IMP_Minus_with_operands_a_b_def split: option.splits)
+  unfolding binary_assign_constant_def
+  apply (rule seq_terminates_when[of 1 "3*n"])
+  apply simp
+   apply (rule result_of_binary_assign_zero)
+  unfolding IMP_State_To_IMP_Minus_def
+  using result_of_binary_assign_constant_bits[of n v x] 
+  by (simp add: fun_eq_iff
+  IMP_State_To_IMP_Minus_with_operands_a_b_def split: option.splits)
 
 lemma result_of_binary_assign_constant_on_translated_state:
   assumes "n > 0"
-  shows "t_small_step_fun (50 * (n + 1)) (binary_assign_constant n v x,
+  shows "t_small_step_fun (50 * (n + 2)) (binary_assign_constant n v x,
     IMP_State_To_IMP_Minus s n)
     = (SKIP, IMP_State_To_IMP_Minus (s(v := x)) n)"
-  apply(rule t_small_step_fun_increase_time[where ?t="3*n"])
+  apply(rule t_small_step_fun_increase_time[where ?t="3*n+2"])
   apply simp
   apply(subst result_of_binary_assign_constant_on_translated_state_aux)
   using assms by auto
@@ -102,11 +170,11 @@ lemma result_of_binary_assign_constant_on_translated_state:
 fun copy_var_to_operand:: "nat \<Rightarrow> char \<Rightarrow> vname \<Rightarrow> IMP_Minus_com" where
 "copy_var_to_operand 0 op v = SKIP" |
 "copy_var_to_operand (Suc i) op v =
-   (IF [var_bit_to_var (v, i)] \<noteq>0 THEN
+   (IF var_bit_to_var (v, i) \<noteq>0 THEN
    (operand_bit_to_var (op, i)) ::= One
     ELSE
     (operand_bit_to_var (op, i)) ::= Zero) ;;
-    copy_var_to_operand i op v "
+    copy_var_to_operand i op v"
 
 lemma copy_var_to_operand_result:
   "t_small_step_fun (4 * n) (copy_var_to_operand n op v, s)
@@ -158,7 +226,7 @@ definition copy_atom_to_operand:: "nat \<Rightarrow> char \<Rightarrow> AExp.ato
   AExp.V x \<Rightarrow> copy_var_to_operand n op x)"
 
 lemma copy_atom_to_operand_a_result:
-  "t_small_step_fun (4 * n) (copy_atom_to_operand n (CHR ''a'') a,
+  "t_small_step_fun (4 * n) (copy_atom_to_operand n (a_chr) a,
    IMP_State_To_IMP_Minus_with_operands_a_b s n b c)
   = (SKIP,  IMP_State_To_IMP_Minus_with_operands_a_b s n (AExp.atomVal a s) c)"
   by(auto simp: copy_atom_to_operand_def fun_eq_iff copy_const_to_operand_result
@@ -167,7 +235,7 @@ lemma copy_atom_to_operand_a_result:
       split!: option.splits AExp.atomExp.splits char.splits bool.splits)
 
 lemma copy_atom_to_operand_b_result:
-  "t_small_step_fun (4 * n) (copy_atom_to_operand n (CHR ''b'') a,
+  "t_small_step_fun (4 * n) (copy_atom_to_operand n (b_chr) a,
    IMP_State_To_IMP_Minus_with_operands_a_b s n b c)
   = (SKIP,  IMP_State_To_IMP_Minus_with_operands_a_b s n b (AExp.atomVal a s))"
   by(auto simp: copy_atom_to_operand_def fun_eq_iff copy_const_to_operand_result
@@ -188,106 +256,197 @@ lemma copy_atom_to_operand_variables:
   by(auto simp: enumerate_variables_def var_bit_to_var_neq_operand_bit_to_var[symmetric])
 
 definition assign_var_carry::
-  "nat \<Rightarrow> vname \<Rightarrow> nat \<Rightarrow> nat \<Rightarrow> nat \<Rightarrow> IMP_Minus_com" where
-"assign_var_carry i v a b c =
+  "nat \<Rightarrow> vname \<Rightarrow> nat \<Rightarrow> nat \<Rightarrow> nat \<Rightarrow> nat \<Rightarrow> IMP_Minus_com" where
+"assign_var_carry i v a b c z =
   (var_bit_to_var (v, i)) ::= (if a + b + c = 1 \<or> a + b + c = 3 then One else Zero) ;;
-  ''carry'' ::= (if a + b + c \<ge> 2 then One else Zero)"
+  carry ::= (if a + b + c \<ge> 2 then One else Zero) ;;
+  zero ::= (if z = 0 \<and> (a + b + c = 0 \<or> a + b + c = 2) then Zero else One)"
 
 lemma result_of_assign_var_carry:
-  "t_small_step_fun 7 (assign_var_carry i v a b c, s)
+  "t_small_step_fun 7 (assign_var_carry i v a b c z, s)
     = (SKIP, s(var_bit_to_var (v, i) \<mapsto> (if a + b + c = 1 \<or> a + b + c = 3 then One else Zero),
-     ''carry'' \<mapsto> (if a + b + c \<ge> 2 then One else Zero)))"
+     carry \<mapsto> (if a + b + c \<ge> 2 then One else Zero),
+      zero \<mapsto> (if z = 0 \<and> (a + b + c = 0 \<or> a + b + c = 2) then Zero else One)))"
   by(auto simp: assign_var_carry_def t_small_step_fun_terminate_iff)
 
 definition full_adder:: "nat \<Rightarrow> vname \<Rightarrow> IMP_Minus_com" where
-"full_adder i v  = (let assign = assign_var_carry i v; op_a = operand_bit_to_var (CHR ''a'', i);
-  op_b = operand_bit_to_var (CHR ''b'', i) in
-  IF [op_a]\<noteq>0 THEN
-    IF [''carry'']\<noteq>0 THEN
-      IF [op_b]\<noteq>0 THEN assign 1 1 1
-      ELSE assign 1 1 0
-    ELSE
-      IF [op_b]\<noteq>0 THEN assign 1 0 1
-      ELSE assign 1 0 0
-  ELSE
-    IF [''carry'']\<noteq>0 THEN
-      IF [op_b]\<noteq>0 THEN assign 0 1 1
-      ELSE assign 0 1 0
-    ELSE
-      IF [op_b]\<noteq>0 THEN assign 0 0 1
-      ELSE assign 0 0 0)"
+"full_adder i v  = (
+let
+  assign = assign_var_carry i v;
+  op_a = operand_bit_to_var (a_chr, i);
+  op_b = operand_bit_to_var (b_chr, i)
+ in
+  IF op_a\<noteq>0 THEN (
+    IF op_b\<noteq>0 THEN (
+      IF carry\<noteq>0 THEN (
+        IF zero\<noteq>0 THEN assign 1 1 1 1
+                      ELSE assign 1 1 1 0)
+      ELSE (
+        IF zero\<noteq>0 THEN assign 1 1 0 1
+                      ELSE assign 1 1 0 0))
+    ELSE (
+      IF carry\<noteq>0 THEN (
+        IF zero\<noteq>0 THEN assign 1 0 1 1
+                      ELSE assign 1 0 1 0)
+      ELSE (
+        IF zero\<noteq>0 THEN assign 1 0 0 1
+                       ELSE assign 1 0 0 0)))
+  ELSE (
+    IF op_b\<noteq>0 THEN (
+      IF carry\<noteq>0 THEN (
+        IF zero\<noteq>0 THEN assign 0 1 1 1
+                      ELSE assign 0 1 1 0)
+      ELSE (
+        IF zero\<noteq>0 THEN assign 0 1 0 1
+                      ELSE assign 0 1 0 0))
+    ELSE (
+      IF carry\<noteq>0 THEN (
+        IF zero\<noteq>0 THEN assign 0 0 1 1
+                      ELSE assign 0 0 1 0)
+      ELSE (
+        IF zero\<noteq>0 THEN assign 0 0 0 1
+                      ELSE assign 0 0 0 0)))
+)"
 
 lemma full_adder_correct:
-  assumes "i = 0 \<longrightarrow> s ''carry'' = Some Zero"
-    "i > 0 \<longrightarrow> s ''carry'' = Some (nth_carry (i - 1) a b)"
-    "s (operand_bit_to_var (CHR ''a'', i)) = Some (nth_bit a i)"
-    "s (operand_bit_to_var (CHR ''b'', i)) = Some (nth_bit b i)"
-  shows "t_small_step_fun 10 (full_adder i v, s) = (SKIP,
-    s(var_bit_to_var (v, i) \<mapsto> nth_bit (a + b) i, ''carry'' \<mapsto> nth_carry i a b))"
+  assumes 
+    "i = 0 \<longrightarrow> s carry = Some Zero \<and> s zero = Some Zero"
+    "i > 0 \<longrightarrow> s carry = Some (nth_carry (i - 1) a b) \<and> s zero = Some (zero_bit (a+b) i)"
+    "s (operand_bit_to_var (a_chr, i)) = Some (nth_bit a i)"
+    "s (operand_bit_to_var (b_chr, i)) = Some (nth_bit b i)"
+  shows "t_small_step_fun 11 (full_adder i v, s) = (SKIP,
+    s(var_bit_to_var (v, i) \<mapsto> nth_bit (a + b) i, carry \<mapsto> nth_carry i a b, zero \<mapsto> zero_bit (a + b) (i + 1)))"
   using assms
   apply(simp add: full_adder_def Let_def t_small_step_fun_terminate_iff result_of_assign_var_carry)
   apply(cases i)
-  by(simp_all add: fun_eq_iff first_bit_of_add nth_bit_of_add)
+   apply (simp_all add: fun_eq_iff first_bit_of_add nth_bit_of_add zero_bit_rec)
+  done
+
+
 
 lemma full_adder_variables: "set (enumerate_variables (full_adder i v)) =
-  { operand_bit_to_var (CHR ''a'', i), operand_bit_to_var (CHR ''b'', i), var_bit_to_var (v, i),
-    ''carry''}"
-  apply (auto simp: full_adder_def Let_def)
-  by(simp_all add: enumerate_variables_def assign_var_carry_def split: if_splits)
+  { operand_bit_to_var (a_chr, i), operand_bit_to_var (b_chr, i), var_bit_to_var (v, i),
+    carry, zero}"
+  apply (subst larvs_set_enum[symmetric])
+  unfolding full_adder_def by (auto simp: Let_def assign_var_carry_def)
 
 lemma sequence_of_full_adders:
   assumes
-    "s ''carry'' = Some Zero"
-    "\<forall>j < k. s (operand_bit_to_var (CHR ''a'', j)) = Some (nth_bit a j)"
-    "\<forall>j < k. s (operand_bit_to_var (CHR ''b'', j)) = Some (nth_bit b j)"
+    "s carry = Some Zero"
+    "s zero = Some Zero"
+    "\<forall>j < k. s (operand_bit_to_var (a_chr, j)) = Some (nth_bit a j)"
+    "\<forall>j < k. s (operand_bit_to_var (b_chr, j)) = Some (nth_bit b j)"
   shows
-   "t_small_step_fun (12 * k) (com_list_to_seq (map (\<lambda>i. full_adder i v) [0..< k]), s)
+   "t_small_step_fun (13 * k) (com_list_to_seq (map (\<lambda>i. full_adder i v) [0..< k]), s)
   = (SKIP, (\<lambda>w. (case var_to_var_bit w of
     Some (w', m) \<Rightarrow> (if w' = v \<and> m < k then Some (nth_bit (a + b) m) else s w) |
-    _ \<Rightarrow> (if w = ''carry'' \<and> k > 0 then Some (nth_carry (k - 1) a b)
+    _ \<Rightarrow> (if w = carry \<and> k > 0 then Some (nth_carry (k-1) a b)
+          else if w = zero then Some (zero_bit (a+b) k)
           else s w))))"
   using assms
 proof(induction k)
   case 0
-  then show ?case by(auto simp: fun_eq_iff split: option.splits)
+  with assms(1,2) show ?case by (auto simp: fun_eq_iff split: option.splits)
 next
   case (Suc k)
-  hence "t_small_step_fun (12 + 12 * k)
-   (com_list_to_seq ((map (\<lambda>i. full_adder i v) [0..< k]) @ [full_adder k v]), s)
-    = (SKIP, (\<lambda>w. (case var_to_var_bit w of
-    Some (w', m) \<Rightarrow> (if w' = v \<and> m < Suc k then Some (nth_bit (a + b) m) else s w) |
-    _ \<Rightarrow> (if w = ''carry'' \<and> Suc k > 0 then Some (nth_carry k a b)
-          else s w))))"
-    apply(auto simp only: com_list_to_seq_of_length_one_terminates_iff
-        intro!: t_small_step_fun_com_list_to_seq_terminates[where ?t1.0="12 * k" and ?t2.0=11])
-    apply(auto)
-    apply(subst full_adder_correct)
-    by(auto simp add: fun_eq_iff var_to_var_bit_eq_Some_iff split!: option.splits)
-  thus ?case by auto
+  let ?s = 
+    "(\<lambda>w. case var_to_var_bit w of
+      Some (w', m) \<Rightarrow> if w' = v \<and> m < k then Some (nth_bit (a + b) m) else s w
+    | None \<Rightarrow> 
+      if w = carry \<and> 0 < k then Some (nth_carry (k - 1) a b) else
+      if w = zero then Some (zero_bit (a + b) k) 
+      else s w)"
+
+  from Suc.prems have
+    "\<forall>j<k. s (operand_bit_to_var (a_chr, j)) = Some (nth_bit a j)"
+    "\<forall>j<k. s (operand_bit_to_var (b_chr, j)) = Some (nth_bit b j)"
+    by auto
+  from Suc.IH[OF Suc.prems(1,2) this] 
+  have 1: "t_small_step_fun (13 * k) (com_list_to_seq (map (\<lambda>i. full_adder i v) [0..<k]), s) = (SKIP, ?s)"
+    by simp
+  let ?s2 =
+    "(\<lambda>w. case var_to_var_bit w of
+      Some (w', m) \<Rightarrow> if w' = v \<and> m < Suc k then Some (nth_bit (a + b) m) else s w
+    | None \<Rightarrow>
+      if w = carry \<and> 0 < Suc k then Some (nth_carry (Suc k - 1) a b) else 
+      if w = zero then Some (zero_bit (a + b) (Suc k))
+      else s w)"
+
+  have 2: "t_small_step_fun 11 ((full_adder k v), ?s) = (SKIP, ?s2)"
+    apply (subst full_adder_correct)
+    by (auto simp: Suc.prems fun_eq_iff var_to_var_bit_eq_Some_iff split!: if_splits option.splits)
+  have "map (\<lambda>i. full_adder i v) [0..<Suc k] = (map (\<lambda>i. full_adder i v) [0..<k]) @ [full_adder k v]" by simp
+  with 1 2 show ?case
+    apply simp
+    apply (rule t_small_step_fun_com_list_to_seq_terminates)
+      apply auto
+    done
 qed
 
+definition write_zero where
+"write_zero n v = 
+  IF zero\<noteq>0 THEN 
+    (var_bit_to_var (v, n)) ::= One
+   ELSE (var_bit_to_var (v, n)) ::= Zero;;
+   carry ::= Zero ;;
+   zero ::= Zero"
+
+lemma result_write_zero: "t_small_step_fun 6
+     (write_zero n v,
+      \<lambda>w. case var_to_var_bit w of
+          None \<Rightarrow>
+            if w = carry \<and> 0 < n then Some cv else
+            if w = zero then Some (zero_bit c n) else
+            IMP_State_To_IMP_Minus_with_operands_a_b s n a b w
+        | Some (w', m) \<Rightarrow> 
+            if w' = v \<and> m < n then Some (nth_bit c m)
+            else IMP_State_To_IMP_Minus_with_operands_a_b s n a b w) =
+    (SKIP,
+     \<lambda>w. case var_to_var_bit w of
+          None \<Rightarrow>
+            if w = carry then Some Zero else
+            if w = zero then Some Zero else
+            IMP_State_To_IMP_Minus_with_operands_a_b s n a b w
+        | Some (w', m) \<Rightarrow>
+            if w' = v \<and> m = n then Some (zero_bit ((s(v := c)) w') m) else 
+            if w' = v \<and> m < n then Some (nth_bit c m)
+            else IMP_State_To_IMP_Minus_with_operands_a_b s n a b w)"
+  unfolding write_zero_def
+  by (auto simp: numeral_eq_Suc simp: fun_eq_iff var_to_var_bit_eq_Some_iff split: if_splits option.splits)
+
+lemma write_zero_vars[simp]: 
+  "set (enumerate_variables (write_zero n v)) = {zero, carry, var_bit_to_var (v,n)}"
+  unfolding write_zero_def
+  apply (subst larvs_set_enum[symmetric])
+  by auto
+
 definition adder:: "nat \<Rightarrow> vname \<Rightarrow> IMP_Minus_com" where
-"adder n v = com_list_to_seq (map (\<lambda>i. full_adder i v) [0..< n]) ;;
-  ''carry'' ::= Zero"
+"adder n v = 
+  com_list_to_seq (map (\<lambda>i. full_adder i v) [0..< n]) ;; 
+  write_zero n v
+"
 
 lemma result_of_adder:
   assumes "a + b < 2 ^ n"
-  shows "t_small_step_fun (12 * n + 2) (adder n v,
+  shows "t_small_step_fun (13 * n + 13) (adder n v,
     IMP_State_To_IMP_Minus_with_operands_a_b s n a b)
     = (SKIP, IMP_State_To_IMP_Minus_with_operands_a_b (s(v := a + b)) n a b)"
+  using assms
   apply(simp only: adder_def)
-  apply(rule seq_terminates_when[OF _  sequence_of_full_adders,
-        where ?t2.0="1" and ?b="''carry'' ::= Zero"])
-  by(auto simp: fun_eq_iff IMP_State_To_IMP_Minus_with_operands_a_b_def
-      split: option.splits)
+  apply(rule seq_terminates_when[OF _  sequence_of_full_adders[where a=a and b=b],of _ 6])
+  apply (auto simp: fun_eq_iff var_to_var_bit_eq_Some_iff IMP_State_To_IMP_Minus_with_operands_a_b_def
+      split!: option.splits if_splits)
+  apply (subst result_write_zero)
+  apply (auto simp: IMP_State_To_IMP_Minus_with_operands_a_b_def split: if_splits option.splits)
+  done
 
 definition binary_adder:: "nat \<Rightarrow> vname \<Rightarrow> AExp.atomExp \<Rightarrow> AExp.atomExp \<Rightarrow> IMP_Minus_com" where
 "binary_adder n v a b =
-  copy_atom_to_operand n (CHR ''a'') a ;;
-  (copy_atom_to_operand n (CHR ''b'') b ;;
+  copy_atom_to_operand n (a_chr) a ;;
+  (copy_atom_to_operand n (b_chr) b ;;
   (adder n v ;;
-  (copy_atom_to_operand n (CHR ''a'') (AExp.N 0) ;;
-  copy_atom_to_operand n (CHR ''b'') (AExp.N 0))))"
+  (copy_atom_to_operand n (a_chr) (AExp.N 0) ;;
+  copy_atom_to_operand n (b_chr) (AExp.N 0))))"
 
 lemma binary_adder_correct:
   assumes "n > 0"
@@ -302,85 +461,115 @@ lemma binary_adder_correct:
   assms
   by(fastforce simp: binary_adder_def IMP_State_To_IMP_Minus_def)
 
+
+section \<open>Subtraction\<close>
+
 definition assign_var_carry_sub::
-  "nat \<Rightarrow> vname \<Rightarrow> nat \<Rightarrow> nat \<Rightarrow> nat \<Rightarrow> IMP_Minus_com" where
-"assign_var_carry_sub i v a b c =
-  (var_bit_to_var (v, i)) ::= (if b + c = 0 \<or> b + c = 2 then (if a = 1 then One else Zero)
-    else (if b + c = 1 \<and> a = 0 then One else Zero)) ;;
-  ''carry'' ::= (if a < b + c then One else Zero)"
+  "nat \<Rightarrow> vname \<Rightarrow> nat \<Rightarrow> nat \<Rightarrow> nat \<Rightarrow> nat \<Rightarrow> IMP_Minus_com" where
+"assign_var_carry_sub i v a b c z =
+  (var_bit_to_var (v, i)) ::= 
+    (if b + c = 0 \<or> b + c = 2 then (if a = 1 then One else Zero)
+     else (if b + c = 1 \<and> a = 0 then One else Zero)) ;;
+  carry ::= (if a < b + c then One else Zero);;
+  zero ::= (if z = 0 \<and> ((a + b + c = 0) \<or> (b + c = 2 \<and> a = 0) \<or> (b + c = 1 \<and> a = 1)) then Zero else One)"
 
 lemma result_of_assign_var_carry_sub:
-  "t_small_step_fun 7 (assign_var_carry_sub i v a b c, s)
+  "t_small_step_fun 7 (assign_var_carry_sub i v a b c z, s)
     = (SKIP, s(var_bit_to_var (v, i) \<mapsto> (if b + c = 0 \<or> b + c = 2 then (if a = 1 then One else Zero)
     else (if b + c = 1 \<and> a = 0 then One else Zero)),
-     ''carry'' \<mapsto>  (if a < b + c then One else Zero)))"
+     carry \<mapsto>  (if a < b + c then One else Zero), 
+     zero \<mapsto> (if z = 0 \<and> ((a + b + c = 0) \<or> (b + c = 2 \<and> a = 0) \<or> (b + c = 1 \<and> a = 1)) then Zero else One)))"
   by(auto simp: assign_var_carry_sub_def t_small_step_fun_terminate_iff)
 
 definition full_subtractor:: "nat \<Rightarrow> vname \<Rightarrow> IMP_Minus_com" where
-"full_subtractor i v  = (let assign = assign_var_carry_sub i v;
-  op_a = [operand_bit_to_var (CHR ''a'', i)];
-  op_b = [operand_bit_to_var (CHR ''b'', i)] in
-  IF op_a\<noteq>0 THEN
-    IF [''carry'']\<noteq>0 THEN
-      IF op_b\<noteq>0 THEN assign 1 1 1
-      ELSE assign 1 1 0
-    ELSE
-      IF op_b\<noteq>0 THEN assign 1 0 1
-      ELSE assign 1 0 0
-  ELSE
-    IF [''carry'']\<noteq>0 THEN
-      IF op_b\<noteq>0 THEN assign 0 1 1
-      ELSE assign 0 1 0
-    ELSE
-      IF op_b\<noteq>0 THEN assign 0 0 1
-      ELSE assign 0 0 0)"
+"full_subtractor i v  = (
+let
+  assign = assign_var_carry_sub i v;
+  op_a = operand_bit_to_var (a_chr, i);
+  op_b = operand_bit_to_var (b_chr, i)
+  in
+  IF op_a\<noteq>0 THEN (
+    IF op_b\<noteq>0 THEN (
+      IF carry\<noteq>0 THEN (
+        IF zero\<noteq>0 THEN assign 1 1 1 1
+                      ELSE assign 1 1 1 0)
+      ELSE (
+        IF zero\<noteq>0 THEN assign 1 1 0 1
+                      ELSE assign 1 1 0 0))
+    ELSE (
+      IF carry\<noteq>0 THEN (
+        IF zero\<noteq>0 THEN assign 1 0 1 1
+                      ELSE assign 1 0 1 0)
+      ELSE (
+        IF zero\<noteq>0 THEN assign 1 0 0 1
+                       ELSE assign 1 0 0 0)))
+  ELSE (
+    IF op_b\<noteq>0 THEN (
+      IF carry\<noteq>0 THEN (
+        IF zero\<noteq>0 THEN assign 0 1 1 1
+                      ELSE assign 0 1 1 0)
+      ELSE (
+        IF zero\<noteq>0 THEN assign 0 1 0 1
+                      ELSE assign 0 1 0 0))
+    ELSE (
+      IF carry\<noteq>0 THEN (
+        IF zero\<noteq>0 THEN assign 0 0 1 1
+                      ELSE assign 0 0 1 0)
+      ELSE (
+        IF zero\<noteq>0 THEN assign 0 0 0 1
+                      ELSE assign 0 0 0 0)))
+)"
 
 lemma full_subtractor_correct_no_underflow:
   assumes "a \<ge> b"
-    "i = 0 \<longrightarrow> s ''carry'' = Some Zero"
-    "i > 0 \<longrightarrow> s ''carry'' = Some (nth_carry_sub (i - 1) a b)"
-    "s (operand_bit_to_var (CHR ''a'', i)) = Some (nth_bit a i)"
-    "s (operand_bit_to_var (CHR ''b'', i)) = Some (nth_bit b i)"
-  shows "t_small_step_fun 10 (full_subtractor i v, s) = (SKIP,
-    s(var_bit_to_var (v, i) \<mapsto> nth_bit (a - b) i, ''carry'' \<mapsto> nth_carry_sub i a b))"
+    "i = 0 \<longrightarrow> s carry = Some Zero \<and> s zero = Some Zero"
+    "i > 0 \<longrightarrow> s carry = Some (nth_carry_sub (i - 1) a b) \<and> s zero = Some (zero_bit (a-b) i)"
+    "s (operand_bit_to_var (a_chr, i)) = Some (nth_bit a i)"
+    "s (operand_bit_to_var (b_chr, i)) = Some (nth_bit b i)"
+  shows "t_small_step_fun 11 (full_subtractor i v, s) = (SKIP,
+    s(var_bit_to_var (v, i) \<mapsto> nth_bit (a - b) i, carry \<mapsto> nth_carry_sub i a b, zero \<mapsto> zero_bit (a - b) (i + 1)))"
   using assms
-  apply(simp add: full_subtractor_def Let_def t_small_step_fun_terminate_iff
-      result_of_assign_var_carry_sub)
+  apply(simp add: full_subtractor_def Let_def t_small_step_fun_terminate_iff result_of_assign_var_carry_sub)
   apply(cases i)
-  by(simp_all add: fun_eq_iff first_bit_of_sub_n_no_underflow nth_bit_of_sub_n_no_underflow Let_def)
+  apply (simp_all add: fun_eq_iff first_bit_of_sub_n_no_underflow nth_bit_of_sub_n_no_underflow Let_def zero_bit_rec)
+  done
 
 lemma full_subtractor_variables: "set (enumerate_variables (full_subtractor i v)) =
-  { operand_bit_to_var (CHR ''a'', i), operand_bit_to_var (CHR ''b'', i), var_bit_to_var (v, i),
-    ''carry''}"
-  apply (auto simp: full_subtractor_def Let_def)
-  by(simp_all add: enumerate_variables_def assign_var_carry_sub_def split: if_splits)
+  { operand_bit_to_var (a_chr, i), operand_bit_to_var (b_chr, i), var_bit_to_var (v, i),
+    carry, zero}"
+  apply (subst larvs_set_enum[symmetric])
+  unfolding full_subtractor_def Let_def
+  by (auto simp: assign_var_carry_sub_def)
 
 lemma sequence_of_full_subtractors_no_underflow:
   assumes "a \<ge> b"
-    "s ''carry'' = Some Zero"
-    "\<forall>j < n. s (operand_bit_to_var (CHR ''a'', j)) = Some (nth_bit a j)"
-    "\<forall>j < n. s (operand_bit_to_var (CHR ''b'', j)) = Some (nth_bit b j)"
+    "s carry = Some Zero"
+    "s zero = Some Zero"
+    "\<forall>j < n. s (operand_bit_to_var (a_chr, j)) = Some (nth_bit a j)"
+    "\<forall>j < n. s (operand_bit_to_var (b_chr, j)) = Some (nth_bit b j)"
   shows
-   "t_small_step_fun (12 * n)
-                       (com_list_to_seq (map (\<lambda>i. full_subtractor i v) [0..< n]), s)
+   "t_small_step_fun (13 * n) (com_list_to_seq (map (\<lambda>i. full_subtractor i v) [0..< n]), s)
   = (SKIP, (\<lambda>w. (case var_to_var_bit w of
     Some (w', m) \<Rightarrow> (if w' = v \<and> m < n then Some (nth_bit (a - b) m) else s w) |
-    _ \<Rightarrow> (if w = ''carry'' \<and> n > 0 then Some (nth_carry_sub (n - 1) a b)
+    _ \<Rightarrow> (if w = carry \<and> n > 0 then Some (nth_carry_sub (n - 1) a b)
+          else if w = zero then Some (zero_bit (a-b) n)
           else s w))))"
   using assms
 proof(induction n)
   case 0
-  then show ?case by(auto simp: fun_eq_iff split: option.splits)
+  with assms(1,2) show ?case by (auto simp: fun_eq_iff split: option.splits)
 next
   case (Suc n)
-  have "t_small_step_fun (12 + 12 * n)
+  have "t_small_step_fun (13 + 13 * n)
    (com_list_to_seq ((map (\<lambda>i. full_subtractor i v) [0..< n]) @ [full_subtractor n v]), s)
     = (SKIP, (\<lambda>w. (case var_to_var_bit w of
-    Some (w', m) \<Rightarrow> (if w' = v \<and> m < Suc n then Some (nth_bit (a - b) m) else s w) |
-    _ \<Rightarrow> (if w = ''carry'' \<and> Suc n > 0 then Some (nth_carry_sub n a b)
-          else s w))))"
+      Some (w', m) \<Rightarrow> (if w' = v \<and> m < Suc n then Some (nth_bit (a - b) m) else s w) |
+      None \<Rightarrow> 
+        (if w = carry \<and> Suc n > 0 then Some (nth_carry_sub n a b) else
+         if w = zero then Some (zero_bit (a-b) (Suc n))
+         else s w))))"
     apply(rule t_small_step_fun_com_list_to_seq_terminates[OF _ Suc.IH
-          iffD2[OF com_list_to_seq_of_length_one_terminates_iff[where ?t="11"]]])
+          iffD2[OF com_list_to_seq_of_length_one_terminates_iff[where ?t="12"]]])
     using Suc  apply(auto)
     apply(subst full_subtractor_correct_no_underflow)
     using Suc
@@ -391,26 +580,28 @@ qed
 lemma sequence_of_full_subtractors_with_underflow:
   assumes "a < b"
     "a < 2^n" "b < 2^n"
-    "s ''carry'' = Some Zero"
-    "\<forall>j < n. s (operand_bit_to_var (CHR ''a'', j)) = Some (nth_bit a j)"
-    "\<forall>j < n. s (operand_bit_to_var (CHR ''b'', j)) = Some (nth_bit b j)"
+    "s carry = Some Zero"
+    "s zero = Some Zero"
+    "\<forall>j < n. s (operand_bit_to_var (a_chr, j)) = Some (nth_bit a j)"
+    "\<forall>j < n. s (operand_bit_to_var (b_chr, j)) = Some (nth_bit b j)"
   shows
-   "t_small_step_fun (12 * n)
-                       (com_list_to_seq (map (\<lambda>i. full_subtractor i v) [0..< n]), s)
+   "t_small_step_fun (13 * n) (com_list_to_seq (map (\<lambda>i. full_subtractor i v) [0..< n]), s)
   = (SKIP, (\<lambda>w. (case var_to_var_bit w of
     Some (w', m) \<Rightarrow> (if w' = v \<and> m < n then Some (nth_bit (2^n + a - b) m) else s w) |
-    _ \<Rightarrow> (if w = ''carry'' \<and> n > 0 then Some One
+    _ \<Rightarrow> (if w = carry \<and> n > 0 then Some One
+          else if w = zero then Some (zero_bit (2^n + a - b) n)
           else s w))))"
 proof -
-  have "\<forall>j < n. s (operand_bit_to_var (CHR ''a'', j)) = Some (nth_bit (2 ^ n + a) j)"
+  have "\<forall>j < n. s (operand_bit_to_var (a_chr, j)) = Some (nth_bit (2 ^ n + a) j)"
     using nth_bit_add_out_of_range[OF \<open>a < 2^n\<close>]
-      \<open>\<forall>j < n. s (operand_bit_to_var (CHR ''a'', j)) = Some (nth_bit a j)\<close> by simp
+      \<open>\<forall>j < n. s (operand_bit_to_var (a_chr, j)) = Some (nth_bit a j)\<close> by simp
   moreover have "2 ^ n + a > b" using \<open>b < 2^n\<close> by simp
-  ultimately have "t_small_step_fun (12 * n)
+  ultimately have "t_small_step_fun (13 * n)
                        (com_list_to_seq (map (\<lambda>i. full_subtractor i v) [0..< n]), s)
   = (SKIP, (\<lambda>w. (case var_to_var_bit w of
     Some (w', m) \<Rightarrow> (if w' = v \<and> m < n then Some (nth_bit (2^n + a - b) m) else s w) |
-    _ \<Rightarrow> (if w = ''carry'' \<and> n > 0 then Some (nth_carry_sub (n - 1) (2^n + a) b)
+    _ \<Rightarrow> (if w = carry \<and> n > 0 then Some (nth_carry_sub (n - 1) (2^n + a) b) else
+          if w = zero then Some (zero_bit (2^n + a - b) n)
           else s w))))"
     using sequence_of_full_subtractors_no_underflow[where ?a="2^n + a" and ?b=b] assms
     by(auto simp: fun_eq_iff)
@@ -418,62 +609,136 @@ proof -
 qed
 
 definition underflow_handler:: "nat \<Rightarrow> vname \<Rightarrow> IMP_Minus_com" where
-"underflow_handler n v = (IF [''carry'']\<noteq>0 THEN (''carry'' ::= Zero ;;
+"underflow_handler n v = (
+IF carry\<noteq>0 THEN 
+  ((carry ::= Zero ;;
+   zero ::= Zero);;
   binary_assign_constant n v 0)
-  ELSE SKIP)"
+ELSE SKIP)"
+
+(* proper setup... why was this not done before ?! *)
+
+lemma seq_intro:
+ "t_small_step_fun n1 (c1,s) = (SKIP,s2) \<Longrightarrow> 
+  t_small_step_fun n2 (c2,s2) = (SKIP,s3) \<Longrightarrow>
+  t = n1 + n2 + 1 \<Longrightarrow>  
+  t_small_step_fun t (c1;;c2,s) = (SKIP,s3)"
+  apply (auto simp add: t_small_step_fun_decomposition t_small_step_fun_small_step_fun tsmall_seq)
+  by (metis IMP_Minus_Small_StepT.small_step_fun.simps(3)
+      t_small_step_fun_decomposition t_small_step_fun_small_step_fun
+      tsmall_seq)
+
+lemma assign_intro:
+"t_small_step_fun (Suc 0) (c ::= b,s) = (SKIP,s(c := Some b))"
+  by simp
+
+lemma ifTrue_intro:
+"s b \<noteq> Some Zero \<Longrightarrow> t_small_step_fun n (c, s) = (SKIP,s2) \<Longrightarrow> n2 = Suc n \<Longrightarrow>
+   t_small_step_fun n2 (IF b\<noteq>0 THEN c ELSE c2,s) = (SKIP, s2)"
+  by simp
+
+lemma ifFalse_intro:
+"s b = Some Zero \<Longrightarrow> t_small_step_fun n (c2, s) = (SKIP,s2) \<Longrightarrow> n2 = Suc n \<Longrightarrow>
+   t_small_step_fun n2 (IF b\<noteq>0 THEN c ELSE c2,s) = (SKIP, s2)"
+  by simp
+
+
+lemmas intros = seq_intro assign_intro 
+
+
+lemma result_underflow_handler_carry: "s carry \<noteq> Some Zero \<Longrightarrow>
+ t_small_step_fun (3 * n + 8)
+     (underflow_handler n v, s) =
+    (SKIP, (\<lambda>w. case var_to_var_bit w of
+          None \<Rightarrow>
+            if w = carry then Some Zero
+            else if w = zero then Some Zero
+            else s w
+          | Some (w', m) \<Rightarrow>
+              if w' = v \<and> m < n then Some (nth_bit 0 m)
+              else if w' = v \<and> m = n then Some (zero_bit 0 m)
+              else s w))"
+  unfolding underflow_handler_def
+  apply (auto  intro!:  intros ifTrue_intro)
+  apply (subst t_small_step_fun_increase_time[OF _ result_of_binary_assign_constant])
+   apply (auto split!: if_splits option.splits)
+  done
+
+lemma result_underflow_handler_carry_Skip: "s carry = Some Zero \<Longrightarrow>
+  t_small_step_fun (3 * n + 8)
+     (underflow_handler n v, s) =
+    (SKIP, s)"
+  unfolding underflow_handler_def
+  by (auto intro!: intros ifFalse_intro)  
 
 definition subtract_handle_underflow::
   "nat \<Rightarrow> vname \<Rightarrow> IMP_Minus_com" where
 "subtract_handle_underflow n v =
   com_list_to_seq (map (\<lambda>i. full_subtractor i v) [0..<n]) ;;
-  underflow_handler n v"
+  (underflow_handler n v;;
+  write_zero n v)"
+
+lemma "Zero = zero_bit 0 n"
+  using zero_bit_one by fastforce
 
 lemma result_of_subtract_handle_underflow:
   assumes "n > 0" "a < 2 ^ n" "b < 2 ^ n"
-  shows "t_small_step_fun (15 * n + 4) (subtract_handle_underflow n v,
+  shows "t_small_step_fun (16 * n + 16) (subtract_handle_underflow n v,
     IMP_State_To_IMP_Minus_with_operands_a_b s n a b)
     = (SKIP, IMP_State_To_IMP_Minus_with_operands_a_b (s(v := a - b)) n a b)"
 proof(cases "a < b")
   case True
-  then show ?thesis
-    apply(simp only: subtract_handle_underflow_def)
-    apply(rule seq_terminates_when[OF _  sequence_of_full_subtractors_with_underflow[where ?a=a and ?b=b],
-          where ?t2.0="3 * n + 3"])
-    using assms apply(auto simp add: underflow_handler_def t_small_step_fun_terminate_iff)
-     apply(auto simp add: t_small_step_fun_small_step_fun result_of_binary_assign_constant fun_eq_iff)
-    by(auto simp:  IMP_State_To_IMP_Minus_with_operands_a_b_of_changed_s_neq_iff
-        var_to_var_bit_eq_Some_iff split!: option.splits if_splits)
+  with assms show ?thesis
+    apply (simp only: subtract_handle_underflow_def)
+    apply (rule seq_terminates_when[OF _  sequence_of_full_subtractors_with_underflow[where ?a=a and ?b=b], of _ "3*n + 15"]) 
+            apply auto
+    apply (rule seq_terminates_when[of "3*n + 8" "6"])
+      apply auto
+    apply (subst result_underflow_handler_carry)
+     apply (auto)
+    unfolding write_zero_def
+    apply (auto  simp: numeral_eq_Suc simp: fun_eq_iff var_to_var_bit_eq_Some_iff IMP_State_To_IMP_Minus_with_operands_a_b_of_changed_s_neq_iff split: if_splits option.splits)
+     defer using zero_bit_one apply fastforce
+    using IMP_State_To_IMP_Minus_with_operands_a_b_of_changed_s_neq_iff
+    by (metis not_Some_eq)
 next
   case False
-  then show ?thesis
+  with assms show ?thesis
     apply(simp only: subtract_handle_underflow_def)
     apply(rule seq_terminates_when[OF _  sequence_of_full_subtractors_no_underflow[where ?a=a and ?b=b],
-          where ?t2.0="3 * n + 3"])
-    using assms apply(auto simp add: underflow_handler_def t_small_step_fun_terminate_iff)
-       apply(auto simp add: t_small_step_fun_small_step_fun result_of_binary_assign_constant fun_eq_iff)
-    using nth_carry_sub_no_underflow[OF _ \<open>a < 2 ^ n\<close> \<open>b < 2 ^ n\<close>]
+          where ?t2.0="3 * n + 15"])
+          apply auto
+    apply (rule seq_terminates_when[of "3*n+8" 6])
+    apply auto
+     apply (subst result_underflow_handler_carry_Skip)
+      apply auto
+    unfolding write_zero_def
+    apply (auto simp: numeral_eq_Suc simp: fun_eq_iff var_to_var_bit_eq_Some_iff IMP_State_To_IMP_Minus_with_operands_a_b_of_changed_s_neq_iff split: if_splits option.splits)
+    apply (metis One_nat_def assms(2,3) nth_carry_sub_no_underflow
+        verit_comp_simplify1(3))
+     using nth_carry_sub_no_underflow[OF _ \<open>a < 2 ^ n\<close> \<open>b < 2 ^ n\<close>]
     apply(auto simp:  IMP_State_To_IMP_Minus_with_operands_a_b_of_changed_s_neq_iff
         var_to_var_bit_eq_Some_iff
         split!: option.splits if_splits)
-    by(auto simp: IMP_State_To_IMP_Minus_with_operands_a_b_def)
+     by(auto simp: IMP_State_To_IMP_Minus_with_operands_a_b_def)
 qed
 
 lemma subtract_handle_underflow_variables:
   "set (enumerate_variables (subtract_handle_underflow n v))
-  = { operand_bit_to_var (op, i) | i op. i < n \<and> (op = CHR ''a'' \<or> op = CHR ''b'') }
+  = { operand_bit_to_var (op, i) | i op. i < n \<and> (op = a_chr \<or> op = b_chr) }
     \<union> { var_bit_to_var (v, i) | i. i < n }
-    \<union> { ''carry'' }"
+    \<union> { carry, zero, var_bit_to_var (v, n) }"
   by(auto simp: subtract_handle_underflow_def
-      set_enumerate_variables_seq com_list_to_seq_variables full_subtractor_variables
-      set_enumerate_variables_if underflow_handler_def binary_assign_constant_variables)
+       set_enumerate_variables_seq com_list_to_seq_variables full_subtractor_variables
+       set_enumerate_variables_if underflow_handler_def)
 
 definition binary_subtractor:: "nat \<Rightarrow> vname \<Rightarrow> AExp.atomExp \<Rightarrow> AExp.atomExp \<Rightarrow> IMP_Minus_com" where
 "binary_subtractor n v a b =
-  copy_atom_to_operand n (CHR ''a'') a ;;
-  (copy_atom_to_operand n (CHR ''b'') b ;;
+  copy_atom_to_operand n (a_chr) a ;;
+  (copy_atom_to_operand n (b_chr) b ;;
   (subtract_handle_underflow n v ;;
-  (copy_atom_to_operand n (CHR ''a'') (AExp.N 0) ;;
-  copy_atom_to_operand n (CHR ''b'') (AExp.N 0))))"
+  (copy_atom_to_operand n (a_chr) (AExp.N 0) ;;
+  copy_atom_to_operand n (b_chr) (AExp.N 0))))"
 
 lemma binary_subtractor_correct:
   assumes "n > 0"
@@ -481,19 +746,20 @@ lemma binary_subtractor_correct:
   shows "t_small_step_fun (50 * (n + 1)) (binary_subtractor n v a b,
     IMP_State_To_IMP_Minus s n)
     = (SKIP, IMP_State_To_IMP_Minus (s(v := AExp.atomVal a s - AExp.atomVal b s)) n)"
-  using seq_terminates_when'[OF copy_atom_to_operand_a_result[where ?n=n]
-      seq_terminates_when'[OF copy_atom_to_operand_b_result
-      seq_terminates_when'[OF result_of_subtract_handle_underflow
-      seq_terminates_when'[OF copy_atom_to_operand_a_result copy_atom_to_operand_b_result]]]]
-  assms
-  by(fastforce simp: binary_subtractor_def IMP_State_To_IMP_Minus_def)
+  unfolding binary_subtractor_def
+  using assms
+  apply (auto simp: IMP_State_To_IMP_Minus_def  intro!: intros copy_atom_to_operand_a_result copy_atom_to_operand_b_result 
+      result_of_subtract_handle_underflow )
+  apply (subst t_small_step_fun_increase_time[OF _ copy_atom_to_operand_b_result])
+   apply auto
+  done
 
 text \<open> The two copy_atom_to_operand which don't have any effect on the output are only a hack to
        ensure that all bits of all variables in IMP occur in IMP- \<close>
 
 fun assign_shifted_bits:: "nat \<Rightarrow> vname \<Rightarrow> IMP_Minus_com" where
 "assign_shifted_bits 0 v = SKIP" |
-"assign_shifted_bits (Suc i) v = (IF [operand_bit_to_var ((CHR ''a''), Suc i)]\<noteq>0 THEN
+"assign_shifted_bits (Suc i) v = (IF operand_bit_to_var ((a_chr), Suc i)\<noteq>0 THEN
     (var_bit_to_var (v, i)) ::= One
   ELSE
     (var_bit_to_var (v, i)) ::= Zero) ;;
@@ -502,30 +768,28 @@ fun assign_shifted_bits:: "nat \<Rightarrow> vname \<Rightarrow> IMP_Minus_com" 
 lemma result_of_assign_shifted_bits:
   "t_small_step_fun (3 * k) (assign_shifted_bits k v, s) = (SKIP, (\<lambda>w.
     (case var_to_var_bit w of Some(v', i) \<Rightarrow> (if v' = v \<and> i < k then
-      (if s (operand_bit_to_var (CHR ''a'', Suc i)) \<noteq> Some Zero then Some One else Some Zero)
+      (if s (operand_bit_to_var (a_chr, Suc i)) \<noteq> Some Zero then Some One else Some Zero)
       else s w) |
       _ \<Rightarrow> s w)))"
 proof(induction k arbitrary: s)
   case (Suc k)
-  have *: "t_small_step_fun 2 (IF [operand_bit_to_var ((CHR ''a''), Suc k)]\<noteq>0 THEN
+  have *: "t_small_step_fun 2 (IF operand_bit_to_var ((a_chr), Suc k)\<noteq>0 THEN
       (var_bit_to_var (v, k)) ::= One
    ELSE
       (var_bit_to_var (v, k)) ::= Zero, s) = (SKIP, s(var_bit_to_var (v, k) \<mapsto>
-        (if s (operand_bit_to_var (CHR ''a'', Suc k)) \<noteq> Some Zero then One else Zero)))"
+        (if s (operand_bit_to_var (a_chr, Suc k)) \<noteq> Some Zero then One else Zero)))"
     by(auto simp: numeral_2_eq_2)
   show ?case
     using seq_terminates_when[OF _ * Suc.IH, where ?t="3 + 3 * k"]
     apply (auto simp: fun_eq_iff var_to_var_bit_eq_Some_iff split: option.splits)
-    using var_bit_to_var_neq_operand_bit_to_var
-    by (metis operand_bit_to_var.simps)+
+    using var_bit_to_var_neq_operand_bit_to_var by (metis operand_bit_to_var.simps)+
 qed (auto simp: fun_eq_iff split: option.splits)
 
 lemma assign_shifted_bits_variables: "set (enumerate_variables (assign_shifted_bits k v))
-  = { var_bit_to_var (v, i) | i. i < k } \<union> { operand_bit_to_var (CHR ''a'', i) | i. i > 0 \<and> i \<le> k }"
+  = { var_bit_to_var (v, i) | i. i < k } \<union> { operand_bit_to_var (a_chr, i) | i. i > 0 \<and> i \<le> k }"
   apply(induction k)
    apply(auto simp: set_enumerate_variables_seq set_enumerate_variables_if)
-  using operand_bit_to_var_eq_operand_bit_to_var_iff'
-  by (metis Suc_eq_plus1 le_SucE)
+  done
 
 definition assignment_to_binary:: "nat \<Rightarrow> vname \<Rightarrow> AExp.aexp \<Rightarrow> IMP_Minus_com" where
 "assignment_to_binary n v aexp = (case aexp of
@@ -551,13 +815,15 @@ qed (auto simp: assignment_to_binary_def)
 
 lemma assignment_to_binary_variables:
   "n > 0 \<Longrightarrow> set (enumerate_variables (assignment_to_binary n v a)) \<subseteq>
-    { var_bit_to_var (w, i) | w i. i < n \<and> (w = v \<or> w \<in> set (vars a)) }
-    \<union> { operand_bit_to_var (op, i) | op i. i < n \<and> (op = CHR ''a'' \<or> op = CHR ''b'') }
-    \<union> { ''carry'' }"
+    { var_bit_to_var (w, i) | w i. i \<le> n \<and> (w = v \<or> w \<in> set (vars a)) }
+    \<union> { operand_bit_to_var (op, i) | op i. i < n \<and> (op = a_chr \<or> op = b_chr) }
+    \<union> { carry, zero }"
   apply(cases a)
-  by(auto simp: assignment_to_binary_def binary_adder_def set_enumerate_variables_seq
+  apply(auto simp: assignment_to_binary_def binary_adder_def set_enumerate_variables_seq
       copy_atom_to_operand_variables adder_def com_list_to_seq_variables full_adder_variables
     binary_subtractor_def subtract_handle_underflow_variables
     split: atomExp.splits)
+  done
+  
 
 end
