IMP-/IMP_To_IMP-/IMP_To_IMP_Minus_State_Translations.thy
@@ -11,21 +11,44 @@ text \<open> We define a translation between IMP states, which map registers to 
        are assumed to be sufficient to represent each natural number in the IMP states, a register
        ''x'' in IMP is represented by n registers in IMP-: ''#$x'', ''##$x'', ... ''#...#$x'',
         where the IMP- register starting with k hashes represents the k- 1th bit of the
-       IMP register. Furthermore, the IMP- states contain special registers ''carry'' and
+       IMP register. Furthermore, the IMP- states contain special registers carry and
         operands ''a'' and ''b'' with n bits respectively, which we will use when replacing
         arithmetic expressions by binary operations when translating IMP to IMP- programs. \<close>
                           
 type_synonym state = IMP_Base.state
 type_synonym bit_state = "IMP_Minus_Base.state"
 
+definition "sep1 = CHR ''#''"
+definition "sep2 = CHR ''$''"
+definition "a_chr = CHR ''a''"
+definition "b_chr = CHR ''b''"
+
+lemma sep1_ne_sep2[simp]: "sep1 \<noteq> sep2" "sep2 \<noteq> sep1"
+  unfolding sep1_def sep2_def by simp_all
+
+lemma sep1_ne_a[simp]: "sep1 \<noteq> a_chr" "a_chr \<noteq> sep1"
+  unfolding sep1_def a_chr_def by simp_all
+
+lemma sep2_ne_a[simp]: "sep2 \<noteq> a_chr" "a_chr \<noteq> sep2"
+  unfolding sep2_def a_chr_def by simp_all
+
+lemma a_ne_b[simp]: "a_chr \<noteq> b_chr" "b_chr \<noteq> a_chr"
+  unfolding a_chr_def b_chr_def by simp_all
+
+lemma sep1_ne_b[simp]: "sep1 \<noteq> b_chr"  "b_chr \<noteq> sep1"
+  unfolding sep1_def b_chr_def by simp_all
+
+lemma sep2_ne_b[simp]: "sep2 \<noteq> b_chr" "b_chr \<noteq> sep2"
+  unfolding sep2_def b_chr_def by simp_all
+
 definition var_to_var_bit:: "vname \<Rightarrow> (vname * nat) option" where
 "var_to_var_bit v =
    (if length v > 0 then
-      (if hd v = CHR ''#'' then
-        (let t = dropWhile (\<lambda>i. i = CHR ''#'') v;
-             l = length (takeWhile (\<lambda>i. i = CHR ''#'') v) - 1
+      (if hd v = sep1 then
+        (let t = dropWhile (\<lambda>i. i = sep1) v;
+             l = length (takeWhile (\<lambda>i. i = sep1) v) - 1
          in
-           (if length t > 0 \<and> hd t = CHR ''$'' then
+           (if length t > 0 \<and> hd t = sep2 then
               Some (tl t, l)
             else
               None))
@@ -33,41 +56,43 @@ definition var_to_var_bit:: "vname \<Rightarrow> (vname * nat) option" where
          None)
     else None)"
 
-fun n_hashes:: "nat \<Rightarrow> string" where
-"n_hashes 0 = []" |
-"n_hashes (Suc n) = (CHR ''#'') # (n_hashes n)"
+definition n_hashes :: "nat \<Rightarrow> string" where "n_hashes n = replicate n (sep1)"
 
 definition var_bit_to_var:: "(vname * nat) \<Rightarrow> vname" where
-"var_bit_to_var vk = (n_hashes (snd vk + 1)) @ ''$''  @ (fst vk)"
+"var_bit_to_var vk = (n_hashes (snd vk + 1)) @ [sep2]  @ (fst vk)"
 
-lemma dropWhile_n_hashes[simp]: "dropWhile (\<lambda>i. i = CHR ''#'') (n_hashes x @ CHR ''$'' # y)
-  = CHR ''$'' # y"
+lemma dropWhile_n_hashes[simp]: "dropWhile (\<lambda>i. i = sep1) (n_hashes x @ sep2 # y)
+  = sep2 # y"
   apply(induction x)
-  by(auto)
+  by(auto simp: n_hashes_def sep1_def sep2_def)
 
 lemma length_takeWhile_n_hashes[simp]:
-  "length (takeWhile (\<lambda>i. i = CHR ''#'') (n_hashes x @ CHR ''$'' # y)) = x"
+  "length (takeWhile (\<lambda>i. i = sep1) (n_hashes x @ sep2 # y)) = x"
   apply(induction x)
-  by auto
+  by (auto simp: n_hashes_def sep1_def sep2_def)
 
-lemma encoded_var_decomposition[simp]: "x \<noteq> [] \<Longrightarrow> hd x = CHR ''#''
-  \<Longrightarrow> hd (dropWhile (\<lambda>i. i = CHR ''#'') x) = CHR ''$''
-  \<Longrightarrow> c \<in> set x \<Longrightarrow> c \<noteq> CHR ''#''
-  \<Longrightarrow> n_hashes (length (takeWhile (\<lambda>i. i = CHR ''#'') x))
-    @ CHR ''$'' # tl (dropWhile (\<lambda>i. i = CHR ''#'') x) = x"
+lemma encoded_var_decomposition[simp]: "x \<noteq> [] \<Longrightarrow> hd x = sep1
+  \<Longrightarrow> hd (dropWhile (\<lambda>i. i = sep1) x) = sep2
+  \<Longrightarrow> c \<in> set x \<Longrightarrow> c \<noteq> sep1
+  \<Longrightarrow> n_hashes (length (takeWhile (\<lambda>i. i = sep1) x))
+    @ sep2 # tl (dropWhile (\<lambda>i. i = sep1) x) = x"
 proof (induction x)
   case (Cons a x)
   hence *: "x \<noteq> []" by auto
-  have "hd x = CHR ''#'' \<or> hd x \<noteq> CHR ''#''" by auto
+  have "hd x = sep1 \<or> hd x \<noteq> sep1" by auto
   thus ?case
     apply(elim disjE)
-    using Cons * apply(auto)
-    by (smt hd_Cons_tl list.size(3) n_hashes.simps(1) self_append_conv2 takeWhile.simps(1)
-        takeWhile_dropWhile_id takeWhile_tail)
+    using Cons * apply(auto simp: n_hashes_def)
+    by (metis (lifting) dropWhile_eq_self_iff list.collapse list.size(3) replicate_empty takeWhile_dropWhile_id
+        takeWhile_eq_Nil_iff)
 qed auto
 
 lemma var_to_var_bit_var_bit_to_var[simp]: "var_to_var_bit (var_bit_to_var x) = Some x"
-  by (auto simp: var_to_var_bit_def var_bit_to_var_def Let_def)
+  unfolding var_to_var_bit_def var_bit_to_var_def Let_def
+  apply (auto simp: var_to_var_bit_def var_bit_to_var_def Let_def)
+  unfolding sep1_def sep2_def n_hashes_def sep1_def sep2_def
+  apply simp_all 
+  done
 
 lemma var_to_var_bit_eq_Some_iff: "var_to_var_bit x = Some y \<longleftrightarrow> x = var_bit_to_var y"
 proof
@@ -75,90 +100,93 @@ proof
   thus "x = var_bit_to_var y"
     apply(auto simp: var_to_var_bit_def var_bit_to_var_def Let_def split: if_splits)
     using encoded_var_decomposition
-    by (smt Nitpick.size_list_simp(2) One_nat_def char.inject length_tl list.expand list.sel(1)
-        list.sel(3) list.simps(3) n_hashes.simps(2) self_append_conv2
-        takeWhile_dropWhile_id tl_append2)
+    by (simp add: takeWhile_eq_Nil_iff)
 qed auto
 
 lemma var_bit_to_var_eq_iff[simp]: "var_bit_to_var (a, b) = var_bit_to_var (c, d) \<longleftrightarrow> (a = c \<and> b = d)"
   apply(auto simp: var_bit_to_var_def)
    apply (metis dropWhile_n_hashes list.inject)
-  by (metis length_takeWhile_n_hashes)
+  by (metis length_takeWhile_n_hashes nat.inject)
 
-lemma var_to_var_bit_of_carry[simp]: "var_to_var_bit ''carry'' = None"
-  by(auto simp: var_to_var_bit_def)
+(* opaque def, otherwise automation tries to work with strings... *)
+definition "zero = ''zero''"
+definition "carry = ''carry''"
 
-lemma var_bit_to_var_neq_carry[simp]: "''carry'' \<noteq> var_bit_to_var (x, y) "
-  by(auto simp: var_bit_to_var_def)
+lemma zero_ne_carry[simp]: "zero \<noteq> carry" "carry \<noteq> zero"
+  unfolding zero_def carry_def by simp_all
 
-lemma var_bit_to_var_neq_carry'[simp]: "var_bit_to_var (x, y) = ''carry'' \<longleftrightarrow> False"
-  by(auto simp: var_bit_to_var_def)
+lemma var_to_var_bit_zero[simp]: "var_to_var_bit zero = None"
+  by(simp add: var_to_var_bit_def zero_def sep1_def)
 
+lemma var_to_var_bit_of_carry[simp]: "var_to_var_bit carry = None"
+  by(auto simp: var_to_var_bit_def carry_def sep1_def)
 
-(*
-fun operand_bit_to_var:: "operand \<Rightarrow> vname" where
-"operand_bit_to_var (a n) = replicate (n + 1) (CHR ''a'')" |
-"operand_bit_to_var (b n) = replicate (n + 1) (CHR ''b'')"
-*)
-fun operand_bit_to_var:: "(char * nat) \<Rightarrow> vname" where
-"operand_bit_to_var (c, 0) = [c]" |
-"operand_bit_to_var (c, (Suc n)) = c # operand_bit_to_var (c, n)"
+lemma var_bit_to_var_neq_carry[simp]: "carry \<noteq> var_bit_to_var (x, y)" "var_bit_to_var (x, y) \<noteq> carry"
+  by(auto simp: var_bit_to_var_def n_hashes_def carry_def sep1_def)
+
+lemma var_bit_to_var_neq_carry'[simp]: "var_bit_to_var (x, y) = carry \<longleftrightarrow> False"
+  by(auto simp: var_bit_to_var_def n_hashes_def carry_def sep1_def)
+
+lemma var_bit_to_var_neq_zero[simp]: "zero \<noteq> var_bit_to_var (x, y)"
+  by(auto simp: var_bit_to_var_def n_hashes_def zero_def sep1_def)
+
+lemma var_bit_to_var_neq_zero'[simp]: "var_bit_to_var (x, y) = zero \<longleftrightarrow> False"
+  by(auto simp: var_bit_to_var_def n_hashes_def zero_def sep1_def)
+
+(* FIXME use def *)
+fun operand_bit_to_var where "operand_bit_to_var (c,n) = replicate (Suc n) c"
+declare operand_bit_to_var.simps[simp del]
+lemmas operand_bit_to_var_def = operand_bit_to_var.simps
 
 definition var_to_operand_bit:: "vname \<Rightarrow> (char * nat) option" where
 "var_to_operand_bit v = (if v \<noteq> [] \<and> v = (operand_bit_to_var (hd v, length v - 1))
   then Some (hd v, length v - 1) else None)"
 
 lemma hd_of_operand_bit_to_var[simp]:
-  "hd (operand_bit_to_var (op, n)) = op" by (induction n) auto
+  "hd (operand_bit_to_var (op, n)) = op" by (induction n) (auto simp: operand_bit_to_var_def)
 
 lemma take_2_of_operand_bit_to_var[simp]:
   "take 2 (operand_bit_to_var (c, k)) = operand_bit_to_var (c, min k 1)"
-  apply (cases k)
-   apply(auto)
-  using hd_of_operand_bit_to_var
-  by (metis lessI less_Suc_eq_0_disj list.discI operand_bit_to_var.simps(1)
-      operand_bit_to_var.simps(2) take0 take_Suc)
+  by (cases k) (auto simp: operand_bit_to_var_def)
 
 lemma length_of_operand_bit_to_var[simp]:
-  "length (operand_bit_to_var (op, n)) = n + 1" by (induction n) auto
+  "length (operand_bit_to_var (op, n)) = n + 1" by (induction n) (auto simp: operand_bit_to_var_def)
 
 lemma var_to_operand_bit_of_operand_bit_to_var[simp]:
   "var_to_operand_bit (operand_bit_to_var (op, n)) = Some (op, n)"
   apply(induction n)
-  by(auto simp: var_to_operand_bit_def)
+  by(auto simp: var_to_operand_bit_def operand_bit_to_var_def)
 
 lemma var_to_operand_bit_eq_Some_iff: "var_to_operand_bit x = Some (op, i)
   \<longleftrightarrow> x = operand_bit_to_var (op, i)"
-  apply(auto simp: var_to_operand_bit_def)
-  apply(cases i)
-  by auto
+  by(auto simp: var_to_operand_bit_def operand_bit_to_var_def)
+  
 
-lemma var_to_operand_bit_of_carry[simp]: "var_to_operand_bit ''carry'' = None"
-  by(simp add: var_to_operand_bit_def)
+lemma var_to_operand_bit_of_zero[simp]: "var_to_operand_bit zero = None"
+  by(simp add: var_to_operand_bit_def zero_def operand_bit_to_var_def)
 
-lemma operand_bit_to_var_neq_carry[simp]: "operand_bit_to_var (op, k) = ''carry'' \<longleftrightarrow> False"
-proof
-  assume "operand_bit_to_var (op, k) = ''carry''"
-  moreover hence "op = CHR ''c''" by (metis hd_of_operand_bit_to_var list.sel)
-  ultimately show False
-    by (metis option.simps var_to_operand_bit_of_carry var_to_operand_bit_of_operand_bit_to_var)
-qed auto
+lemma var_to_operand_bit_of_carry[simp]: "var_to_operand_bit carry = None"
+  by(simp add: var_to_operand_bit_def carry_def operand_bit_to_var_def)
+
+lemma operand_bit_to_var_neq_carry[simp]: "operand_bit_to_var (op, k) = carry \<longleftrightarrow> False"
+  by (metis option.distinct(1) var_to_operand_bit_eq_Some_iff var_to_operand_bit_of_carry)
+
+lemma operand_bit_to_var_neq_zero[simp]: "operand_bit_to_var (op, k) = zero \<longleftrightarrow> False"
+  by (metis option.distinct(1) var_to_operand_bit_of_operand_bit_to_var var_to_operand_bit_of_zero)
 
 lemma set_of_operand_bit_to_var[simp]: "set (operand_bit_to_var (op, b)) = { op }"
-  by (induction b) auto
+  by (induction b) (auto simp: operand_bit_to_var_def)
 
 lemma var_to_operand_bit_var_bit_to_var[simp]: "var_to_operand_bit (var_bit_to_var (a, b)) = None"
-  apply(simp add: var_to_operand_bit_def var_bit_to_var_def)
-  apply(rule ccontr)
-  apply simp
-  apply(drule arg_cong[where ?f=set])
-  by simp
+  unfolding var_to_operand_bit_def var_bit_to_var_def n_hashes_def
+  apply (auto simp: operand_bit_to_var_def)
+  by (metis in_set_conv_decomp in_set_replicate sep1_ne_sep2 set_ConsD)
 
 lemma var_to_var_bit_operand_bit_to_var[simp]: "var_to_var_bit (operand_bit_to_var (c, k)) = None"
   by (simp add: var_to_var_bit_def)
 
 lemma operand_bit_to_var_non_empty: "operand_bit_to_var (op, n) \<noteq> []"
-  by (induction n) auto
+  by (induction n) (auto simp: operand_bit_to_var_def)
 
 lemma operand_bit_to_var_eq_operand_bit_to_var_iff[simp]:
   "operand_bit_to_var (op, a) = operand_bit_to_var (op', b)
@@ -174,28 +202,29 @@ lemma operand_bit_to_var_eq_operand_bit_to_var_iff'[simp]:
   "op # operand_bit_to_var (op, i) = operand_bit_to_var (op', j)
     \<longleftrightarrow> (op = op' \<and> i + 1 = j)"
 proof -
-  have "op # operand_bit_to_var (op, i) =  operand_bit_to_var (op, i + 1)" by simp
-  thus ?thesis using operand_bit_to_var_eq_operand_bit_to_var_iff by presburger
+  have "op # operand_bit_to_var (op, i) =  operand_bit_to_var (op, i + 1)" by (simp add: operand_bit_to_var_def)
+  thus ?thesis using operand_bit_to_var_eq_operand_bit_to_var_iff by metis
 qed
 
 lemma var_bit_to_var_neq_operand_bit_to_var[simp]:
   "var_bit_to_var (v, a) \<noteq> operand_bit_to_var (op, b)"
-proof(rule ccontr)
-  assume "\<not> (var_bit_to_var (v, a) \<noteq> operand_bit_to_var (op, b))"
-  hence "set (var_bit_to_var (v, a)) = set (operand_bit_to_var (op, b))" by simp
-  thus False using set_of_operand_bit_to_var by(auto simp: var_bit_to_var_def)
-qed
+  by (metis option.distinct(1) var_to_var_bit_operand_bit_to_var var_to_var_bit_var_bit_to_var)
+
 
 definition IMP_State_To_IMP_Minus_with_operands_a_b::
   "state \<Rightarrow> nat \<Rightarrow> nat \<Rightarrow> nat \<Rightarrow> bit_state" where
 "IMP_State_To_IMP_Minus_with_operands_a_b s n a b = (\<lambda>v.
   (case var_to_var_bit v of
-     Some (v', k) \<Rightarrow> if k < n then Some (nth_bit (s v') k) else None |
+     Some (v', k) \<Rightarrow> 
+       if k < n then Some (nth_bit (s v') k)
+       else if k = n then Some (zero_bit (s v') k)
+       else None |
      None \<Rightarrow>
        (case var_to_operand_bit v of
-          Some (CHR ''a'', k) \<Rightarrow> if k < n then Some (nth_bit a k) else None |
-          Some (CHR ''b'', k) \<Rightarrow> if k < n then Some (nth_bit b k) else None |
-          _ \<Rightarrow> (if v = ''carry'' then Some Zero else None))))"
+          Some (c, k) \<Rightarrow> if k < n \<and> c = a_chr then Some (nth_bit a k) else
+                         if k < n \<and> c = b_chr then Some (nth_bit b k) else
+                         None |
+          _ \<Rightarrow> (if v = carry \<or> v = zero then Some Zero else None))))"
 
 definition IMP_State_To_IMP_Minus:: "state \<Rightarrow> nat \<Rightarrow> bit_state" where
 "IMP_State_To_IMP_Minus s n
@@ -211,45 +240,48 @@ definition IMP_State_To_IMP_Minus_partial::
            else
              (if k < r then
                 ((\<lambda>x. Some (nth_bit x k)) \<circ>\<^sub>m s) v'
+              else if k = r then
+                ((\<lambda>x. Some (zero_bit x k)) \<circ>\<^sub>m s) v'
               else
                 Some Zero)
         | None \<Rightarrow> (case var_to_operand_bit v of
-            Some (CHR ''a'', k) \<Rightarrow>
-              if k < n then
+            Some (c, k) \<Rightarrow>
+              if c = a_chr \<and> k < n then
+                Some Zero
+              else if c = b_chr \<and> k < n then 
                 Some Zero
               else
-                None
-          | Some (CHR ''b'', k) \<Rightarrow>
-              if k < n then
-                Some Zero
-              else
-                None
+                 None
           |  _ \<Rightarrow>
-              if v = ''carry'' then
+              if v = carry \<or> v = zero then
                 Some Zero
               else
                 None)))"
 
 lemma IMP_State_To_IMP_Minus_partial_of_operand_bit_to_var:
   "IMP_State_To_IMP_Minus_partial s n r (operand_bit_to_var (op, k)) =
-    (if (op = CHR ''a'' \<or> op = CHR ''b'') \<and> k < n then Some Zero else None)"
-  by(auto simp: IMP_State_To_IMP_Minus_partial_def split!: char.splits bool.splits)
+    (if (op = a_chr \<or> op = b_chr) \<and> k < n then Some Zero else None)"
+  unfolding IMP_State_To_IMP_Minus_partial_def by auto
 
 lemma IMP_State_To_IMP_Minus_with_operands_a_b_of_carry[simp]:
-  "IMP_State_To_IMP_Minus_with_operands_a_b s k a b ''carry'' = Some Zero"
+  "IMP_State_To_IMP_Minus_with_operands_a_b s k a b carry = Some Zero"
+  by(auto simp: IMP_State_To_IMP_Minus_with_operands_a_b_def)
+
+lemma IMP_State_To_IMP_Minus_with_operands_a_b_of_zero[simp]:
+  "IMP_State_To_IMP_Minus_with_operands_a_b s k a b zero = Some Zero"
   by(auto simp: IMP_State_To_IMP_Minus_with_operands_a_b_def)
 
 lemma IMP_State_To_IMP_Minus_with_operands_a_b_of_operand_a[simp]:
   "j < k \<Longrightarrow> IMP_State_To_IMP_Minus_with_operands_a_b s k a b
-  (operand_bit_to_var (CHR ''a'', j)) = Some (nth_bit a j)"
+  (operand_bit_to_var (a_chr, j)) = Some (nth_bit a j)"
   by(auto simp: IMP_State_To_IMP_Minus_with_operands_a_b_def)
 
 lemma IMP_State_To_IMP_Minus_with_operands_a_b_of_operand_a'[simp]:
   "j + 1 < k \<Longrightarrow> IMP_State_To_IMP_Minus_with_operands_a_b s k a b
-  (CHR ''a'' # operand_bit_to_var (CHR ''a'', j)) = Some (nth_bit a (j + 1))"
+  (a_chr # operand_bit_to_var (a_chr, j)) = Some (nth_bit a (j + 1))"
 proof-
   assume "j + 1 < k"
-  moreover have "CHR ''a'' # operand_bit_to_var (CHR ''a'', j) = operand_bit_to_var (CHR ''a'', j + 1)"
+  moreover have "a_chr # operand_bit_to_var (a_chr, j) = operand_bit_to_var (a_chr, j + 1)"
     by simp
   ultimately show ?thesis
     using IMP_State_To_IMP_Minus_with_operands_a_b_of_operand_a by presburger
@@ -257,24 +289,41 @@ qed
 
 lemma IMP_State_To_IMP_Minus_with_operands_a_b_of_operand_b[simp]:
   "j < k \<Longrightarrow> IMP_State_To_IMP_Minus_with_operands_a_b s k a b
-  (operand_bit_to_var (CHR ''b'', j)) = Some (nth_bit b j)"
-  by(auto simp: IMP_State_To_IMP_Minus_with_operands_a_b_def)
+  (operand_bit_to_var (b_chr, j)) = Some (nth_bit b j)"
+  by (auto simp: IMP_State_To_IMP_Minus_with_operands_a_b_def)
 
 lemma IMP_State_To_IMP_Minus_with_operands_a_b_of_var_bit_to_var[simp]:
   "IMP_State_To_IMP_Minus_with_operands_a_b s n a b (var_bit_to_var (v, i))
-    = (if i < n then Some (nth_bit (s v) i) else None)"
+    = (if i < n then Some (nth_bit (s v) i) else if i = n then Some (zero_bit (s v) n) else None)"
   by(auto simp: IMP_State_To_IMP_Minus_with_operands_a_b_def)
+
+lemma IMP_State_To_IMP_Minus_with_operands_a_b_of_z[simp]:
+  "n = i \<Longrightarrow> IMP_State_To_IMP_Minus_with_operands_a_b s n a b (var_bit_to_var (v, i))
+    = Some (zero_bit (s v) n)"
+  by(auto simp: IMP_State_To_IMP_Minus_with_operands_a_b_def)
+
+lemma zero_IMP_State_To_IMP_Minus_with_operands_a_b[simp]:
+  "IMP_State_To_IMP_Minus_with_operands_a_b s n a b (var_bit_to_var (v, n)) = Some Zero 
+  \<longleftrightarrow> zero_bit (s v) n = Zero"
+  by(auto simp: IMP_State_To_IMP_Minus_with_operands_a_b_def split: option.splits)
+
+lemma zero_IMP_State_To_IMP_Minus_with_operands_a_b2[simp]:
+  "IMP_State_To_IMP_Minus_with_operands_a_b s n a b (var_bit_to_var (v, n)) = Some One 
+  \<longleftrightarrow> zero_bit (s v) n = One"
+  by(auto simp: IMP_State_To_IMP_Minus_with_operands_a_b_def split: option.splits)
+
 
 lemma IMP_State_To_IMP_Minus_with_operands_a_b_of_changed_s_neq_iff:
   "IMP_State_To_IMP_Minus_with_operands_a_b s n a b x \<noteq>
        IMP_State_To_IMP_Minus_with_operands_a_b (s(v := y)) n a b x
-  \<longleftrightarrow> (\<exists>i < n. var_to_var_bit x = Some (v, i) \<and> nth_bit(s v) i \<noteq> nth_bit y i)"
+  \<longleftrightarrow> (var_to_var_bit x = Some (v, n) \<and> zero_bit (s v) n \<noteq> zero_bit y n) \<or> 
+      (\<exists>i < n. var_to_var_bit x = Some (v, i) \<and> nth_bit(s v) i \<noteq> nth_bit y i)" (is "?lhs \<longleftrightarrow> ?rhs")
   by(auto simp: IMP_State_To_IMP_Minus_with_operands_a_b_def split: option.splits)
 
 lemma dom_of_IMP_State_To_IMP_Minus: "dom (IMP_State_To_IMP_Minus s n) =
-  { ''carry'' }
-  \<union> { var_bit_to_var (w, i) | w i. i < n }
-  \<union> { operand_bit_to_var (op, i) | op i. i < n \<and> (op = CHR ''a'' \<or> op = CHR ''b'') }" for s n
+  { carry, zero }
+  \<union> { var_bit_to_var (w, i) | w i. i \<le> n }
+  \<union> { operand_bit_to_var (op, i) | op i. i < n \<and> (op = a_chr \<or> op = b_chr) }" for s n
   by (auto simp: IMP_State_To_IMP_Minus_def var_to_operand_bit_eq_Some_iff
                  var_to_var_bit_eq_Some_iff IMP_State_To_IMP_Minus_with_operands_a_b_def
            split: char.splits option.splits bool.splits if_splits)
@@ -293,6 +342,18 @@ lemma nth_bit_of_IMP_Minus_State_To_IMP:
     else Zero)"
   by(auto simp: IMP_Minus_State_To_IMP_def split: option.splits)
 
+lemma zero_bit_le[simp]: "a + b < 2 ^ n \<Longrightarrow> zero_bit (a+b) (Suc n) = zero_bit (a+b) n"
+  by (auto simp: zero_bit_def bits_zero_iff less_Suc_eq nth_bit_nat_is_right_shift)
+
+lemma zero_IMP_Minus_State_To_IMP[simp]:
+  "s b < 2 ^n \<Longrightarrow> (IMP_State_To_IMP_Minus s n) (var_bit_to_var (b, n)) = Some Zero \<longleftrightarrow> s b = 0"
+  by (auto simp: IMP_State_To_IMP_Minus_def all_bits_equal_then_equal zero_bit_zero split: option.splits)
+
+lemma zero_IMP_Minus_State_To_IMP2[simp]:
+  "s b < 2 ^n \<Longrightarrow> (IMP_State_To_IMP_Minus s n) (var_bit_to_var (b, n)) = Some One \<longleftrightarrow> s b \<noteq> 0"
+  using all_bits_equal_then_equal
+  by (fastforce simp: IMP_State_To_IMP_Minus_def  zero_bit_one)
+  
 lemma all_bits_geq_k_Zero_then_IMP_Minus_State_To_IMP_range_limited:
   assumes "\<forall>i v. i \<ge> k \<longrightarrow> s (var_bit_to_var (v, i)) \<noteq> Some One"
   shows "finite (range (IMP_Minus_State_To_IMP s n))"
